theories/bool3.v
@@ -1,0 +1,66 @@
+Inductive bool3 : Type :=
+  | TRUE
+  | FALSE
+  | IDK.
+
+Definition and3 (v1 v2 : bool3) :=
+  match v1, v2 with
+  | FALSE, _ => FALSE
+  | _, FALSE => FALSE
+  | TRUE, TRUE => TRUE
+  | _, _ => IDK
+  end.
+
+Definition or3 (v1 v2 : bool3) :=
+  match v1, v2 with
+  | TRUE, _ => TRUE
+  | _, TRUE => TRUE
+  | FALSE, FALSE => FALSE
+  | _, _ => IDK
+  end.
+
+Definition not3 (v : bool3) :=
+  match v with
+  | TRUE => FALSE
+  | FALSE => TRUE
+  | IDK => IDK
+  end.
+
+Inductive bexpr : Type :=
+  | Cst (v : bool3)
+  | Var (n : nat)
+  | And (b1 b2 : bexpr)
+  | Or (b1 b2 : bexpr)
+  | Not (b : bexpr).
+
+Definition of_bool (b : bool) :=
+  if b then TRUE else FALSE.
+
+Fixpoint eval (env : nat -> bool) (b : bexpr) :=
+  match b with
+  | Cst v => v
+  | Var n => of_bool (env n)
+  | And b1 b2 => and3 (eval env b1) (eval env b2)
+  | Or b1 b2 => or3 (eval env b1) (eval env b2)
+  | Not b => not3 (eval env b)
+  end.
+
+Lemma and3_IDK:
+  forall v1 v2,
+    and3 v1 v2 = IDK ->
+    (v1 = IDK /\ v2 = TRUE) \/
+    (v1 = TRUE /\ v2 = IDK) \/
+    (v1 = IDK /\ v2 = IDK).
+Proof.
+  intros [] []; simpl; intuition.
+Qed.
+
+Lemma or3_IDK:
+  forall v1 v2,
+    or3 v1 v2 = IDK ->
+    (v1 = IDK /\ v2 = FALSE) \/
+    (v1 = FALSE /\ v2 = IDK) \/
+    (v1 = IDK /\ v2 = IDK).
+Proof.
+  intros [] []; simpl; intuition.
+Qed.
